improve pre/post-condition automation

theories/Basics/HeterogeneousRelations.v
@@ -1,3 +1,4 @@
+Require Import Coq.Logic.EqdepFacts.
 Require Import ExtLib.Structures.Functor.
 Require Import ExtLib.Structures.Applicative.
 Require Import ExtLib.Structures.Monad.
@@ -20,6 +21,17 @@ Notation Rel A B := (A -> B -> Prop).
 Notation PostRel E1 E2 := (forall (e1 : E1) (e2 : E2), encodes e1 -> encodes e2 -> Prop).
 
 Notation rcompose RR1 RR2 := (rel_compose RR2 RR1).
+
+Definition TruePreRel  {A B} : Rel A B := fun _ _ => True.
+Definition FalsePreRel {A B} : Rel A B := fun _ _ => False.
+Definition eqPreRel {A} : Rel A A := eq.
+
+Definition TruePostRel  {E1 E2} `{EncodingType E1} `{EncodingType E2} :
+  PostRel E1 E2 := fun _ _ _ _ => True.
+Definition FalsePostRel {E1 E2} `{EncodingType E1} `{EncodingType E2} :
+  PostRel E1 E2 := fun _ _ _ _ => False.
+Definition eqPostRel {E} `{EncodingType E} : PostRel E E :=
+  fun e1 e2 a1 a2 => eq_dep1 _ _ e1 a1 e2 a2.
 
 Variant SumPostRel {E1 E2 D1 D2} `{EncodingType E1} `{EncodingType E2} `{EncodingType D1} `{EncodingType D2}
         (RPost1 : PostRel E1 E2) (RPost2 : PostRel D1 D2) : PostRel (E1 + D1) (E2 + D2) :=
